coupling: partial update to use inset_flows.v

coupling_inv.v
@@ -1,4 +1,4 @@
-(** Verification of lock couling template algorithm *)
+(** Verification of lock coupling template algorithm *)
 
 From iris.algebra Require Import excl auth gmap agree gset.
 From iris.heap_lang Require Export lifting notation locations lang.
@@ -38,18 +38,23 @@ Section Coupling_Cameras.
 
   Instance subG_keysetΣ {Σ} : subG keysetΣ Σ → keysetG Σ.
   Proof. solve_inG. Qed.
-  
+
+  (* RA for set of contents *)
+  Class contentG Σ :=
+    ContentG { content_inG :> inG Σ (authR (optionUR (exclR (gsetR K)))) }.
+  Definition contentΣ : gFunctors :=
+    #[GFunctor (authR (optionUR (exclR (gsetR K))))].
+
 End Coupling_Cameras.
 
 (** Verification of the template *)
 Section Coupling_Template.
 
-  Context `{!heapG Σ, !flowintG Σ, !nodesetG Σ, !keysetG Σ} (N : namespace).
+  Context `{!heapG Σ, !flowintG Σ, !nodesetG Σ, !keysetG Σ, !contentG Σ} (N : namespace).
   Notation iProp := (iProp Σ).
 
-  (** The code of the couling template. *)
+  (** The code of the coupling template. *)
 
-  
   Inductive dOp := memberOp | insertOp | deleteOp.
 
   (* The following parameters are the implementation-specific helper functions
@@ -58,7 +63,6 @@ Section Coupling_Template.
 
   Parameter findNext : val.
   Parameter decisiveOp : (dOp → val).
-  Parameter searchStrSpec : (dOp → val).
   Parameter lockLoc : Node → loc.
   Parameter getLockLoc : val.
   Parameter alloc : val.
@@ -68,38 +72,39 @@ Section Coupling_Template.
       let: "l" := getLockLoc "x" in
       if: CAS "l" #false #true
       then #()
-      else "lockN" "x" .
-  
+      else "lockN" "x".
+
   Definition unlockNode : val :=
     λ: "x",
     let: "l" := getLockLoc "x" in
     "l" <- #false.
-  
-  Definition traverse : val :=  
+
+  Definition traverse : val :=
     rec: "tr" "p" "n" "k" :=
       match: (findNext "n" "k") with
         NONE => ("p", "n")
       | SOME "n'" =>
         lockNode "n'";; unlockNode "p";; "tr" "n" "n'" "k"
       end.
-  
-  Definition searchStrOp (Ψ: dOp) (first: Node) : val :=
+
+  Definition CSSOp (Ψ: dOp) (first: Node) : val :=
     λ: "k",
     lockNode #first;;
-             let: "n0" := (findNext #first "k") in
-             match: "n0" with 
-               NONE => ""
-             | SOME "n0" =>
-               lockNode "n0";;
-               let: "pn" := traverse #first "n0" "k" in
-               let: "p" := Fst "pn" in
-               let: "n" := Snd "pn" in
-               let: "m" := alloc #() in
-               let: "res" := (decisiveOp Ψ) "p" "n" "k" in
-               unlockNode "p";; unlockNode "n";; "res" end.
+    let: "n0" := (findNext #first "k") in
+    match: "n0" with
+      NONE => ""
+    | SOME "n0" =>
+      lockNode "n0";;
+      let: "pn" := traverse #first "n0" "k" in
+      let: "p" := Fst "pn" in
+      let: "n" := Snd "pn" in
+      let: "m" := alloc #() in
+      let: "res" := (decisiveOp Ψ) "p" "n" "k" in
+      unlockNode "p";; unlockNode "n";; "res" end.
 
 
-  (** Assumptions on the implementation made by the template proofs. Matching definitions can be found in GRASShopper file list-coupling.spl *)
+  (** Assumptions on the implementation made by the template proofs.
+   * Matching definitions can be found in GRASShopper file list-coupling.spl *)
 
   (* The node predicate is specific to each template implementation. *)
   Parameter node : Node → Node → inset_flowint_ur K → gset K → iProp.
@@ -116,8 +121,8 @@ Section Coupling_Template.
 
   (* TODO: can we get rid of the following? *)
   Instance ccm_ms : CCM (@K_multiset K _ _) := @K_multiset_ccm K _ _.
-  
-  
+
+
   (* The node-local invariant. See list-coupling.spl for the corresponding GRASShopper definition.*)
   (*Definition nodeinv n first I_n  C_n : Prop :=
     C_n = keyset K I_n n ∧ (n = first → ∀ k, k ∈ KS → in_outsets K k I_n).    *)
@@ -128,15 +133,17 @@ Section Coupling_Template.
     ∧ (n = root → ∀ k : K, k ∈ KS → in_outsets K k I_n).
 
   (* The following hypotheses are proved as GRASShopper lemmas in list-coupling.spl *)
-  Hypothesis node_implies_nodeinv : ∀ n I_n C first, (⌜✓I_n⌝)%I ∗ node n first I_n C -∗ node n first I_n C 
-                                                                                      ∗ (⌜nodeinv n first I_n C⌝)%I. 
+  Hypothesis node_implies_nodeinv : ∀ n I_n C first,
+    (⌜✓I_n⌝)%I ∗ node n first I_n C
+    -∗ node n first I_n C ∗ (⌜nodeinv first n I_n C⌝)%I.
 
-  Hypothesis node_sep_star: ∀ n I_n I_n' C C' first, node n first I_n C ∗ node n first I_n' C' -∗ False.
-                                                                     (* change node n first I C → node first n I C*)
+  Hypothesis node_sep_star: ∀ n I_n I_n' C C' first,
+      node n first I_n C ∗ node n first I_n' C' -∗ False.
+  (* TODO change node n first I C → node first n I C*)
 
   Hypothesis contextualLeq_impl_globalinv :
     ∀ I I' first, globalinv K first I → contextualLeq K_multiset I I' → globalinv K first I'.
-        
+
   Lemma successor_not_first : ∀ (I I1 I2 I3 : flowintT) C root n k,
       globalinv K root I →
       I = I1 ⋅ I2 ⋅ I3 →
@@ -164,7 +171,7 @@ Section Coupling_Template.
     pose proof (I_inf_out root) as (root_out & _).
     assert (root = root) by reflexivity.
     pose proof (root_out H k) as root_out_k.
-    
+
     assert (default 0 (inf I n !! k) ≠ 0).
     rewrite e.
     unfold inset, dom_ms, nzmap_dom in root_out_k.
@@ -181,7 +188,7 @@ Section Coupling_Template.
     simpl.
     naive_solver.
     pose proof (lookup_op _ _ (inf I n) (out I1 n) k) as inf_I23_def.
-    
+
     rewrite IDef in inf_I23_def.
     unfold cmra_op, flowintRA, cmra_car, nzmap_total_lookup in inf_I23_def.
     unfold ccm_op, lift_ccm in n_inf_I23.
@@ -190,7 +197,7 @@ Section Coupling_Template.
     rewrite <- n_inf_I23 in inf_I23_def.
     unfold cmra_op, flowintRA, cmra_car in IDef.
     rewrite <- IDef in inf_I23_def.
-    
+
     pose proof (inf_I2 n n_in_I2) as n_inf_I2.
     pose proof (lookup_op _ _ (inf (I2 ⋅ I3) n) (out I3 n) k) as inf_I2_def.
     unfold cmra_op, flowintRA, cmra_car, nzmap_total_lookup in inf_I2_def.
@@ -198,7 +205,7 @@ Section Coupling_Template.
     unfold K_multiset_ccm, ccm_op, lift_ccm in n_inf_I2.
     rewrite <- n_inf_I2 in inf_I2_def.
     rewrite inf_I23_def in inf_I2_def.
-  
+
     assert (default 0 (out I1 n !! k) ≠ 0).
     unfold outset, dom_ms, nzmap_dom in k_in_out1.
     apply elem_of_dom in k_in_out1.
@@ -254,8 +261,8 @@ Section Coupling_Template.
   Parameter findNext_spec : ∀ first (n: Node) (I_n : inset_flowint_ur K) (C: gset K) (k: K),
       ({{{ node n first I_n C ∗ ⌜in_inset K k I_n n⌝ }}}
            findNext #n #k
-       {{{ (b: bool) (n': Node), 
-              RET (match b with true => (SOMEV #n') | false => NONEV end); 
+       {{{ (b: bool) (n': Node),
+              RET (match b with true => (SOMEV #n') | false => NONEV end);
                node n first I_n C ∗ (match b with true => ⌜in_outset K k I_n n'⌝ |
                                           false => ⌜¬in_outsets K k I_n⌝ ∗ ⌜n ≠ first⌝ end) }}})%I.
 
@@ -265,7 +272,7 @@ Section Coupling_Template.
            decisiveOp dop #p #n #k
        {{{ (C_p' C_n' C_m': gset K) (I_p' I_n' I_m': flowintUR K_multiset) (res: bool), RET  #res;
                            node p first I_p' C_p' ∗ node n first I_n' C_n' ∗ node m first I_m' C_m'
-                         ∗ ⌜Ψ dop k (C_p ∪ C_n) (C_p' ∪ C_n' ∪ C_m') res⌝ 
+                         ∗ ⌜Ψ dop k (C_p ∪ C_n) (C_p' ∪ C_n' ∪ C_m') res⌝
                          ∗ ⌜contextualLeq _ (I_p ⋅ I_n) (I_p' ⋅ I_n' ⋅ I_m')⌝
                          ∗ ⌜domm I_p' = {[p]}⌝ ∗ ⌜domm I_n' = {[n]}⌝ ∗ ⌜domm I_m' = {[m]}⌝
                          ∗ ⌜C_p' ⊆ keyset K I_p' p⌝ ∗ ⌜C_n' ⊆ keyset K I_n' n⌝ ∗ ⌜C_m' ⊆ keyset K I_m' m⌝
@@ -273,7 +280,7 @@ Section Coupling_Template.
                          ∗ ⌜keyset K I_m' m ## keyset K I_n' n⌝ ∗ ⌜C_p' ## C_n'⌝ ∗ ⌜C_m' ## C_n'⌝ ∗ ⌜C_p' ## C_m'⌝
                          ∗ ⌜keyset K I_p' p ∪ keyset K I_n' n ∪ keyset K I_m' m = keyset K I_p p ∪ keyset K I_n n⌝ }}})%I.
 
-  Parameter alloc_spec : 
+  Parameter alloc_spec :
       ({{{ True }}}
            alloc #()
        {{{ (m: Node) (l:loc), RET #m; hrep_spatial m ∗ ⌜lockLoc m = l⌝ ∗ l ↦ #false }}})%I.
@@ -284,19 +291,21 @@ Section Coupling_Template.
   Definition cssN : namespace := N .@ "css".
 
   Definition css_inv (γ γ_fp γ_k γ_c : gname) root : iProp :=
-    (∃ I (C: gset K),
+    (∃ (I: inset_flowint_ur K) (C: gsetO K),
         own γ_k (● prod (KS, C)) ∗ own γ (● I) ∗ ⌜globalinv K root I⌝
-        ∗ own γ_fp (● domm I) ∗ own γ_c (● (Some ((Excl C)))) (* <- issue is here *)
+        ∗ own γ_fp (● domm I)
+        ∗ own γ_c (● (Some (Excl C)))
         ∗ ([∗ set] n ∈ (domm I), (∃ b: bool,
-          (lockLoc n) ↦ #b ∗ if b then True
-                             else (∃ (I_n: inset_flowint_ur K) (C_n: gset K),
-                                      own γ (◯ I_n) ∗ ⌜domm I_n = {[n]}⌝ ∗ node n root I_n C_n 
-                                      ∗ own γ_k (◯ prod (keyset K I_n n, C_n)))))
+          (lockLoc n) ↦ #b
+          ∗ if b then True
+            else (∃ (I_n: inset_flowint_ur K) (C_n: gset K),
+                 own γ (◯ I_n) ∗ ⌜domm I_n = {[n]}⌝ ∗ node n root I_n C_n
+                 ∗ own γ_k (◯ prod (keyset K I_n n, C_n)))))
     )%I.
 
   Definition css (γ γ_fp γ_k γ_c : gname) root : iProp :=
     inv N (css_inv γ γ_fp γ_k γ_c root).
-  
+
   Definition css_cont (γ_c: gname) (C: gset K) : iProp :=
     (own γ_c (◯ (Some ((Excl C)))))%I.
 
@@ -309,16 +318,16 @@ Section Coupling_Template.
     apply bi.sep_timeless; try apply _.
     destruct x2; try apply _.
   Qed.
-  
+
   (** Assorted useful lemmas *)
 
-  Lemma globalinv_root_fp: ∀ I root, globalinv root I → root ∈ domm I.
-  Proof. 
+  Lemma globalinv_root_fp: ∀ I root, globalinv K root I → root ∈ domm I.
+  Proof.
     intros I root Hglob. unfold globalinv in Hglob.
     destruct Hglob as [H1 [H2 H3]]. done.
-  Qed.    
+  Qed.
 
-  Lemma auth_set_incl γ_fp Ns Ns' :
+  Lemma auth_set_incl (γ_fp: gname) (Ns: gsetUR Node) Ns' :
     own γ_fp (◯ Ns) ∗ own γ_fp (● Ns') -∗ ⌜Ns ⊆ Ns'⌝.
   Proof.
     rewrite -own_op. rewrite own_valid. iPureIntro.
@@ -328,13 +337,15 @@ Section Coupling_Template.
     apply to_agree_inj in H1. set_solver.
   Qed.
 
-  Lemma auth_own_incl γ (x y: flowintUR) : own γ (● x) ∗ own γ (◯ y) -∗ ⌜y ≼ x⌝.
+  Lemma auth_own_incl γ (x y: inset_flowint_ur K) :
+    own γ (● x) ∗ own γ (◯ y) -∗ ⌜y ≼ x⌝.
   Proof.
     rewrite -own_op. rewrite own_valid. iPureIntro.
     apply auth_both_valid.
   Qed.
 
-  Lemma auth_own_incl_ks γ (x y: keysetUR) : own γ (● x) ∗ own γ (◯ y) -∗ ⌜y ≼ x⌝.
+  Lemma auth_own_incl_ks γ (x y: keysetUR K) :
+    own γ (● x) ∗ own γ (◯ y) -∗ ⌜y ≼ x⌝.
   Proof.
     rewrite -own_op. rewrite own_valid. iPureIntro. rewrite auth_valid_discrete.
     simpl. intros H. destruct H. destruct H0 as [a Ha]. destruct Ha as [Ha Hb].
@@ -363,9 +374,10 @@ Section Coupling_Template.
   Qed.
 
   Lemma flowint_update_result γ I I_n I_n' x :
-    ⌜flowint_update_P I I_n I_n' x⌝ ∧ own γ x -∗
-                       ∃ I', ⌜contextualLeq I I'⌝ ∗ ⌜∃ I_o, I = I_n ⋅ I_o ∧ I' = I_n' ⋅ I_o⌝ 
-                                ∗ own γ (● I' ⋅ ◯ I_n').
+    ⌜flowint_update_P K_multiset I I_n I_n' x⌝ ∧ own γ x -∗
+    ∃ I', ⌜contextualLeq K_multiset I I'⌝
+          ∗ ⌜∃ I_o, I = I_n ⋅ I_o ∧ I' = I_n' ⋅ I_o⌝
+          ∗ own γ (● I' ⋅ ◯ I_n').
   Proof.
     unfold flowint_update_P.
     case_eq (auth_auth_proj x); last first.
@@ -378,7 +390,7 @@ Section Coupling_Template.
       iSplit. iPureIntro. apply H4.
       assert (Auth (auth_auth_proj x) (auth_frag_proj x) = x) as Hx.
       { destruct x. reflexivity. }
-      assert (x = (Auth (Some (1%Qp, to_agree(I'))) (I_n'))) as H'. 
+      assert (x = (Auth (Some (1%Qp, to_agree(I'))) (I_n'))) as H'.
       { rewrite <-Hx. rewrite H. rewrite <-H2. rewrite Hp. rewrite H1.
        rewrite H0. reflexivity. }
       assert (● I' = Auth (Some (1%Qp, to_agree(I'))) ε) as HI'. { reflexivity. }
@@ -387,11 +399,11 @@ Section Coupling_Template.
       { rewrite /(⋅) /=. rewrite left_id. done. }
       assert (Some (1%Qp, to_agree I') ⋅ None = Some (1%Qp, to_agree I')) as Hs.
       { rewrite /(⋅) /=.
-        rewrite /(cmra_op (optionR (prodR fracR (agreeR flowintUR))) (Some (1%Qp, to_agree I')) (None)) /=.
+        rewrite /(cmra_op (optionR (prodR fracR (agreeR (inset_flowint_ur K)))) (Some (1%Qp, to_agree I')) (None)) /=.
         reflexivity. }
       assert (● I' ⋅ ◯ I_n' = (Auth (Some (1%Qp, to_agree(I'))) (I_n'))) as Hd.
       { rewrite /(● I') /= /(◯ I_n') /=. rewrite /(⋅) /=.
-        rewrite /(cmra_op (authR flowintUR) (Auth (Some (1%Qp, to_agree I')) ε) (Auth None I_n')) /=.
+        rewrite /(cmra_op (authR (inset_flowint_ur K)) (Auth (Some (1%Qp, to_agree I')) ε) (Auth None I_n')) /=.
         rewrite /auth_op /=. rewrite HeIn. rewrite Hs. reflexivity. }
       iEval (rewrite Hd). iEval (rewrite <- H'). done.
   Qed.
@@ -411,7 +423,7 @@ Section Coupling_Template.
     iMod "AU" as (b) "[Hb HAU]". iDestruct "Hl" as %Hl.
     iEval (rewrite Hl) in "Hb". destruct b.
     - wp_cmpxchg_fail. iDestruct "HAU" as "[HAU _]".
-      iEval (rewrite Hl) in "HAU". 
+      iEval (rewrite Hl) in "HAU".
       iMod ("HAU" with "Hb") as "H".
       iModIntro. wp_pures. iApply "IH".
       iEval (rewrite <-Hl) in "H". done.
@@ -439,7 +451,7 @@ Section Coupling_Template.
 
   (** Proof of the lock-coupling template *)
 
-  Lemma traverse_spec (γ γ_fp γ_k γ_c: gname) first (k: K) (p n: Node) (Ns: gset Node) I_p C_p I_n C_n:
+  Lemma traverse_spec (γ γ_fp γ_k γ_c: gname) (first: Node) (k: K) (p n: Node) (Ns: gset Node) I_p C_p I_n C_n:
     css γ γ_fp γ_k γ_c first -∗
     {{{ own γ_fp (◯ Ns) ∗ ⌜p ∈ Ns⌝ ∗ ⌜n ∈ Ns⌝ ∗ ⌜first ∈ Ns⌝ ∗ ⌜n ≠ first⌝
         ∗ node p first I_p C_p ∗ own γ (◯ I_p) ∗ ⌜domm I_p = {[p]}⌝ ∗  ⌜in_inset K k I_p p⌝ ∗ ⌜in_outset K k I_p n⌝
@@ -447,22 +459,27 @@ Section Coupling_Template.
         ∗ own γ_k (◯ prod (keyset K I_n n, C_n))
     }}}
       traverse #p #n #k @ ⊤
-    {{{ (p' n': Node) (Ns': gsetUR Node) (I_p' I_n': flowintUR) (C_p' C_n': gset K), 
+    {{{ (p' n': Node) (Ns': gsetUR Node) (I_p' I_n': inset_flowint_ur K) (C_p' C_n': gset K),
         RET (#p', #n');
-        own γ_fp (◯ Ns') ∗ ⌜p' ∈ Ns'⌝ ∗ ⌜n' ∈ Ns'⌝ ∗ own γ (◯ I_p') ∗ ⌜domm I_p' = {[p']}⌝ ∗ own γ (◯ I_n') 
+        own γ_fp (◯ Ns') ∗ ⌜p' ∈ Ns'⌝ ∗ ⌜n' ∈ Ns'⌝ ∗ own γ (◯ I_p') ∗ ⌜domm I_p' = {[p']}⌝ ∗ own γ (◯ I_n')
         ∗ ⌜domm I_n' = {[n']}⌝ ∗ node p' first I_p' C_p' ∗ node n' first I_n' C_n' ∗ ⌜n' ≠ first⌝
         ∗ own γ_k (◯ prod (keyset K I_p' p', C_p'))
-        ∗ own γ_k (◯ prod (keyset K I_n' n', C_n')) 
+        ∗ own γ_k (◯ prod (keyset K I_n' n', C_n'))
         ∗ ⌜in_inset K k I_p' p'⌝ ∗ ⌜in_outset K k I_p' n'⌝ ∗ ⌜¬in_outsets K k I_n'⌝
     }}}.
   Proof.
-    iIntros "#HInv". iIntros (Φ) "!# H HCont". iLöb as "IH" forall (Ns p n I_p I_n C_p C_n). 
+    iIntros "#HInv". iIntros (Φ) "!# H HCont". iLöb as "IH" forall (Ns p n I_p I_n C_p C_n).
     iDestruct "H" as "(#Hfp & % & % & % & % & Hnodep & HIp & % & % & % & Hksp & Hnoden & HIn & % & Hksn)".
-    wp_lam. wp_pures. wp_bind (findNext _ _)%E. 
+    wp_lam. wp_pures. wp_bind (findNext _ _)%E.
     iPoseProof ((own_op γ (◯ I_p) (◯ I_n)) with "[HIp HIn]") as "H"; first by eauto with iFrame.
     iPoseProof (own_valid with "H") as "%". rewrite -auth_frag_op in H7.
     assert (✓ (I_p ⋅ I_n)). { apply (auth_frag_valid (◯ (I_p ⋅ I_n))). done. }
-    assert (in_inset K k I_n n). { apply (inset_monotone I_p I_n k p n); try done. set_solver. }
+    assert (in_inset K k I_n n).
+    { unfold in_inset. fold (inset K I_n n).
+      assert (∀ I1 I2 k n, ✓ (I1 ⋅ I2) → n ∈ domm I2 → k ∈ outset K I1 n → k ∈ inset K I2 n)
+        as outset_impl_inset.
+      { admit. }                (* Need to prove this like flowint_linkset_step in linkset_flows.v *)
+      apply (outset_impl_inset I_p I_n k n); try done. set_solver. }
     iDestruct "H" as "(HIp & HIn)".
     wp_apply ((findNext_spec first n I_n C_n k) with "[Hnoden]"). iFrame "∗ % #".
     iIntros (b n') "(Hnoden & Hb)". destruct b.
@@ -476,10 +493,11 @@ Section Coupling_Template.
       assert (✓ I_n) as HInv. { apply (auth_frag_valid (◯ I_n)). done. }
       assert (✓ I0) as HI0. { apply (auth_auth_valid (I0)). done. }
       assert (n' ∈ domm I2). { apply (flowint_step I0 I_n I2 k n' first); try done. }
-      assert (n' ∈ domm I0). { apply flowint_comp_fp in H12. set_solver. done. }
+      assert (n' ∈ domm I0).
+      { rewrite H12. rewrite flowint_comp_fp. set_solver. rewrite <-H12. done. }
       iMod (own_update γ_fp (● (domm I0)) (● (domm I0) ⋅ ◯ (domm I0)) with "HFP") as "H".
       apply auth_update_core_id. apply gset_core_id. done.
-      iDestruct "H" as "(HFP & #Hfp0)". 
+      iDestruct "H" as "(HFP & #Hfp0)".
       rewrite (big_sepS_elem_of_acc _ (domm I0) n'); last by eauto.
       iDestruct "Hstar" as "[Hb Hstar]".
       iDestruct "Hb" as (b) "[Hlock Hb]".
@@ -491,12 +509,15 @@ Section Coupling_Template.
       iPoseProof ((own_op γ (◯ I_n) (◯ I_n' )) with "[HIn HIn']") as "H"; first by eauto with iFrame.
       iPoseProof (own_valid with "H") as "%". rewrite -auth_frag_op in H18.
       assert (✓ (I_n ⋅ I_n')). { apply (auth_frag_valid (◯ (I_n ⋅ I_n'))). done. }
-      iEval (rewrite -auth_frag_op) in "H". 
+      iEval (rewrite -auth_frag_op) in "H".
       iPoseProof (auth_own_incl with "[$HInt $H]") as (I3)"%".
-      iAssert (node n' first I_n' C_n' ∗ ⌜nodeinv n' first I_n' C_n'⌝)%I with "[Hnoden']" as "(Hnoden' & %)". 
+      iAssert (node n' first I_n' C_n' ∗ ⌜nodeinv first n' I_n' C_n'⌝)%I with "[Hnoden']" as "(Hnoden' & %)".
       { iApply (node_implies_nodeinv _ _ _). iFrame "∗ # %". iPureIntro.
-        apply cmra_valid_op_r in H19. done. } 
-      assert (n' ≠ first) as Hnotf'. { apply (successor_not_first I0 I_n I_n' I3 first n' k C_n'); try done. }
+        apply cmra_valid_op_r in H19. done. }
+      assert (n' ≠ first) as Hnotf'.
+      { apply (successor_not_first I0 I_n I_n' I3 C_n' first n' k); try done.
+        admit.                  (* TODO how to prove k ∈ KS? *)
+      }
       iModIntro. iSplitL "HKS HInt HFP Hcont Hstar Hlock".
       { iNext. iExists I0, C0. iFrame "∗ # %". iApply "Hstar".
       iExists true. iFrame. } iDestruct "H" as "(HIn & HIn')". iIntros "Hc".
@@ -515,20 +536,20 @@ Section Coupling_Template.
       rewrite (big_sepS_elem_of_acc _ (domm I1) p); last by eauto.
       iDestruct "Hstar" as "[Hb Hstar]". iDestruct "Hb" as (b) "[Hlock Hb]".
       destruct b; last first. { iDestruct "Hb" as (In1 Cn1) "(_ & _ & Hrep' & _)".
-      iAssert (⌜False⌝)%I with "[Hrep' Hnodep]" as %Hf. { iApply (node_sep_star p In1 I_p _ _ first). 
+      iAssert (⌜False⌝)%I with "[Hrep' Hnodep]" as %Hf. { iApply (node_sep_star p In1 I_p _ _ first).
       iFrame. } exfalso. done. }
-      iAaccIntro with "Hlock". { iIntros. iModIntro. iFrame "∗ # %". iNext. iExists I1, C1.  
+      iAaccIntro with "Hlock". { iIntros. iModIntro. iFrame "∗ # %". iNext. iExists I1, C1.
       iFrame "∗ # %". iApply "Hstar". iExists true. iFrame. }
       iMod (own_update γ_fp (● (domm I1)) (● (domm I1) ⋅ ◯ (domm I1)) with "HFP") as "H".
       apply auth_update_core_id. apply gset_core_id. done.
-      iDestruct "H" as "(HFP & #Hfp1)". 
+      iDestruct "H" as "(HFP & #Hfp1)".
       iIntros "Hlock". iModIntro. iSplitL "HKS HInt HFP Hcont Hstar Hlock Hnodep HIp Hksp".
       iNext. iExists I1, C1. iFrame "∗ # %". iApply "Hstar". iExists false. iFrame.
       iExists I_p, C_p. iFrame "∗ # %". iIntros "Hc". wp_pures. iSpecialize ("IH" $! (domm I1) n n' I_n I_n' C_n C_n').
-      iApply ("IH" with "[-Hc]"). iFrame "∗ # %". iNext. done. 
+      iApply ("IH" with "[-Hc]"). iFrame "∗ # %". iNext. done.
     - wp_pures. iDestruct "Hb" as "(% & %)". iSpecialize ("HCont" $! p n Ns I_p I_n C_p C_n).
       iApply "HCont". iFrame "∗ # %".
-  Qed.
+  Admitted.
 
   Lemma ghost_update_keyset γ_k dop k Cn Cn' res K1 C:
           ⌜Ψ dop k Cn Cn' res⌝ ∗ own γ_k (● prod (KS, C)) ∗ own γ_k (◯ prod (K1, Cn))
@@ -540,7 +561,7 @@ Section Coupling_Template.
   Theorem searchStrOp_spec (γ γ_fp γ_k γ_c: gname) first (k: K) (dop: dOp):
     ⌜k ∈ KS⌝ ∗ css γ γ_fp γ_k γ_c first -∗
     <<< ∀ (C: gset K), css_cont γ_c C >>>
-      searchStrOp dop first #k @ ⊤ ∖ ↑N
+      CSSOp dop first #k @ ⊤ ∖ ↑N
     <<< ∃ C' (res: bool), css_cont γ_c C' ∗ ⌜Ψ dop k C C' res⌝, RET #res >>>.
   Proof.
     iIntros "(% & #HInv)". iIntros (Φ) "AU". wp_lam. wp_bind (lockNode _)%E.
@@ -561,10 +582,9 @@ Section Coupling_Template.
     iPoseProof (auth_own_incl with "[$HInt $HIf]") as (Io)"%".
     iModIntro. iSplitR "AU HIf Hnodef HCf". iNext. iExists I0, C0. iFrame "∗ # %".
     iApply "Hstar". iExists true. iFrame "∗ # %".
-    wp_pures. wp_bind(findNext _ _)%E. 
+    wp_pures. wp_bind(findNext _ _)%E.
     assert (in_inset K k If first). { unfold globalinv in H0. destruct H0 as [? [? [? ?]]].
-    specialize (H6 first). destruct H6 as [H6 _]. apply (inset_monotone I0 If Io k first); try done.
-    set_solver. apply H6. done. }
+    specialize (H6 first). destruct H6 as [H6 _]. apply (inset_monotone I0 If Io k first); try done; set_solver. }
     wp_apply ((findNext_spec first first If Cf k) with "[Hnodef]").
     { iFrame "∗ # %". } iIntros (b n) "(Hnodef & Hb)".
     destruct b; last first. wp_pures. iDestruct "Hb" as "(% & %)".
@@ -574,8 +594,9 @@ Section Coupling_Template.
     iPoseProof (own_valid with "HInt") as "%". rename H7 into Hcheck.
     assert (✓ I2) as HI2. { apply (auth_auth_valid (I2)). done. }
     iPoseProof (auth_own_incl with "[$HInt $HIf]") as (Io')"%". assert (n ∈ domm I2).
-    { assert (n ∈ domm Io'). { apply (flowint_step I2 If Io' k n first); try done. }
-      apply flowint_comp_fp in H7. set_solver. done. }
+    { assert (n ∈ domm Io').
+      { apply (flowint_step I2 If Io' k n first); try done. }
+      rewrite H7. rewrite flowint_comp_fp. set_solver. rewrite <-H7. done. }
     rewrite (big_sepS_elem_of_acc _ (domm I2) n); last by eauto.
     iDestruct "Hstar" as "[Hb Hstar]".
     iDestruct "Hb" as (b) "[Hlock Hb]".
@@ -591,20 +612,21 @@ Section Coupling_Template.
     iPoseProof ((own_op γ (◯ If) (◯ In)) with "[HIf HIn]") as "H"; first by eauto with iFrame.
     iPoseProof (own_valid with "H") as "%". rewrite -auth_frag_op in H11.
     assert (✓ (If ⋅ In)). { apply (auth_frag_valid (◯ (If ⋅ In))). done. }
-    iEval (rewrite -auth_frag_op) in "H". 
+    iEval (rewrite -auth_frag_op) in "H".
     iPoseProof (auth_own_incl with "[$HInt $H]") as (Iu)"%".
-    iAssert (node n first In Cn ∗ ⌜nodeinv n first In Cn⌝)%I with "[Hnoden]" as "(Hnoden & %)". 
+    iAssert (node n first In Cn ∗ ⌜nodeinv first n In Cn⌝)%I with "[Hnoden]" as "(Hnoden & %)".
     { iApply (node_implies_nodeinv n In Cn first). iFrame "∗ # %". iPureIntro.
-      apply cmra_valid_op_r in H12. done. }  iDestruct "H" as "(HIf & HIn)". 
-    assert (n ≠ first). { apply (successor_not_first I2 If In Iu first n k Cn); try done. }             
+      apply cmra_valid_op_r in H12. done. }  iDestruct "H" as "(HIf & HIn)".
+    assert (n ≠ first).
+    { apply (successor_not_first I2 If In Iu Cn first n k); try done. }
     iModIntro. iSplitR "AU HIf HCf Hnodef HIn Hnoden HCn". { iNext. iExists I2, C2.
     iFrame "∗ # %". iApply "Hstar". iExists true. iFrame. }
-    wp_pures. wp_bind (traverse _ _ _)%E. 
+    wp_pures. wp_bind (traverse _ _ _)%E.
     wp_apply ((traverse_spec γ γ_fp γ_k γ_c first k first n (domm I2) If Cf In Cn)
-                 with "[] [HIf HCf Hnodef HIn HCn Hnoden]"). 
+                 with "[] [HIf HCf Hnodef HIn HCn Hnoden]").
     done. iFrame "∗ # %".
     iIntros (p' n' Ns Ip' In' Cp' Cn') "(#HNs & % & % & HIp' & % & HIn' & % & Hnodep' & Hnoden'
-                        & % & Hksp' & Hksn' & % & % & %)".  
+                        & % & Hksp' & Hksn' & % & % & %)".
     wp_pures. wp_apply (alloc_spec); first done.
     iIntros (m lm) "(Hrepm & % & Hlm)". wp_pures. wp_bind (decisiveOp _ _ _ _)%E.
     iApply fupd_wp. iInv "HInv" as ">H".
@@ -613,13 +635,13 @@ Section Coupling_Template.
     iDestruct "Hstar" as "(Hm & Hstar)". iDestruct "Hm" as (b) "(Hlockm & Hb)".
     iEval (rewrite H24) in "Hlockm". iDestruct (mapsto_valid_2 with "Hlm Hlockm") as "%".
     exfalso. done. }
-    assert (first ∈ domm I3). { apply globalinv_root_fp. done. } 
+    assert (first ∈ domm I3). { apply globalinv_root_fp. done. }
     assert (m ≠ first). { set_solver. }
     iModIntro. iSplitL "HKS HInt HFP Hcont Hstar". iNext.
-    iExists I3, C3. iFrame "∗ # %". iModIntro.    
-    wp_apply ((decisiveOp_insert_spec dop first p' n' m k Ip' In' Cp' Cn') 
+    iExists I3, C3. iFrame "∗ # %". iModIntro.
+    wp_apply ((decisiveOp_insert_spec dop first p' n' m k Ip' In' Cp' Cn')
           with "[Hnodep' Hnoden' Hrepm]"). { iFrame "∗ % #". }
-    iIntros (Cp'' Cn'' Cm'' Ip'' In'' Im'' res) "(Hnodep' & Hnoden' & Hnodem' & % & % & % & H)".  
+    iIntros (Cp'' Cn'' Cm'' Ip'' In'' Im'' res) "(Hnodep' & Hnoden' & Hnodem' & % & % & % & H)".
     iDestruct "H" as "(% & % & % & % & % & % & % & % & % & % & % & %)".
     iApply fupd_wp. iInv "HInv" as ">H".
     iDestruct "H" as (I4 C4) "(HKS & HInt & % & HFP & Hcont & Hstar)".
@@ -628,15 +650,15 @@ Section Coupling_Template.
 
     (* ------ keyset update -------*)
 
-    iPoseProof ((own_op γ_k (◯ prod (keyset K Ip' p', Cp')) (◯ prod (keyset K In' n', Cn')) 
+    iPoseProof ((own_op γ_k (◯ prod (keyset K Ip' p', Cp')) (◯ prod (keyset K In' n', Cn'))
                       with "[Hksp' Hksn']")) as "H"; first by eauto with iFrame.
     assert (◯ prod (keyset K Ip' p', Cp') ⋅ ◯ prod (keyset K In' n', Cn') =
                ◯ (prod (keyset K Ip' p', Cp') ⋅ prod (keyset K In' n', Cn'))).
     { apply (auth_frag_op (prod (keyset K Ip' p', Cp')) (prod (keyset K In' n', Cn'))). }
-    iEval (rewrite H44) in "H". iPoseProof (own_valid with "H") as "%". 
+    iEval (rewrite H44) in "H". iPoseProof (own_valid with "H") as "%".
     assert (✓ (prod (keyset K Ip' p', Cp') ⋅ prod (keyset K In' n', Cn'))).
     { apply (auth_frag_valid (◯ (prod (keyset K Ip' p', Cp') ⋅ prod (keyset K In' n', Cn')))). done. }
-    unfold op,prodOp in H46. repeat case_decide; 
+    unfold op,prodOp in H46. repeat case_decide;
         [ simpl | try exfalso; eauto | try exfalso; eauto | try exfalso; eauto | try exfalso; eauto].
     assert (prod (keyset K Ip'' p', Cp'') ⋅ prod (keyset K In'' n', Cn'') ⋅ prod (keyset K Im'' m, Cm'')
                  = prod (keyset K Ip'' p' ∪ keyset K In'' n' ∪ keyset K Im'' m, Cp'' ∪ Cn'' ∪ Cm'')).
@@ -644,42 +666,49 @@ Section Coupling_Template.
       exfalso. apply H57. set_solver by eauto. exfalso. apply H55. set_solver by eauto. }
     assert (◯ (prod (keyset K Ip'' p', Cp'') ⋅ prod (keyset K In'' n', Cn'') ⋅ prod (keyset K Im'' m, Cm''))
                  = ◯ (prod (keyset K Ip'' p' ∪ keyset K In'' n' ∪ keyset K Im'' m, Cp'' ∪ Cn'' ∪ Cm''))).
-    { rewrite H51. reflexivity. }            
-    assert ((prod (keyset K Ip' p', Cp') ⋅ prod (keyset K In' n', Cn')) 
+    { rewrite H51. reflexivity. }
+    assert ((prod (keyset K Ip' p', Cp') ⋅ prod (keyset K In' n', Cn'))
                   = prod (keyset K Ip' p' ∪ keyset K In' n', Cp' ∪ Cn')).
     { unfold op, prodOp. repeat case_decide; try done. }
     iPoseProof ((own_op γ (◯ Ip') (◯ In')) with "[HIp' HIn']") as "H'"; first by eauto with iFrame.
     iPoseProof (own_valid with "H'") as "%". rewrite -auth_frag_op in H54.
     assert (✓ (Ip' ⋅ In')). { apply (auth_frag_valid (◯ (Ip' ⋅ In'))). done. }
-    assert (in_inset K k In' n'). { apply (inset_monotone Ip' In' k p' n'); try done. set_solver. }
-    assert (k ∈ keyset K In' n'). { apply keyset K_def; try done. } 
-    iMod ((ghost_update_keyset K γ_k dop k (Cp' ∪ Cn') (Cp'' ∪ Cn'' ∪ Cm'') res 
+    assert (in_inset K k In' n'). {
+      assert (∀ I1 I2 k n, ✓ (I1 ⋅ I2) → n ∈ domm I2 → k ∈ outset K I1 n → k ∈ inset K I2 n)
+        as outset_impl_inset.
+      { admit. }                (* Need to prove this like flowint_linkset_step in linkset_flows.v *)
+      apply (outset_impl_inset Ip' In' k n'); try done. set_solver. }
+    assert (k ∈ keyset K In' n'). { apply keyset_def; try done. }
+    iMod ((ghost_update_keyset γ_k dop k (Cp' ∪ Cn') (Cp'' ∪ Cn'' ∪ Cm'') res
                  (keyset K Ip' p' ∪ keyset K In' n') C4) with "[HKS H]") as "Hgks".
-    iEval (rewrite H53) in "H". iFrame "∗ # %". iPureIntro. 
+    iEval (rewrite H53) in "H". iFrame "∗ # %". iPureIntro.
     split. rewrite <-H42. set_solver by eauto. set_solver by eauto.
     iDestruct "Hgks" as (C4') "(% & HKS & H)". iEval (rewrite <-H42) in "H".
     iAssert (own γ_k (◯ (prod (keyset K Ip'' p', Cp'') ⋅ prod (keyset K In'' n', Cn'') ⋅ prod (keyset K Im'' m, Cm''))))
           with "[H]" as "Hv". { iEval (rewrite H52). done. }
     iDestruct "Hv" as "((Hksp' & Hksn') & Hksm')".
-    iMod (auth_update γ_c (C4') with "Hcont Hc") as "[Hcont Hc]".    
+    iMod (auth_update γ_c (C4') with "Hcont Hc") as "[Hcont Hc]".
 
-    (* ------ interface update -------*)  
+    (* ------ interface update -------*)
 
-    iPoseProof (own_valid with "HInt") as "%". 
-    iMod (own_updateP (flowint_update_P I4 (Ip' ⋅ In') (Ip'' ⋅ In'' ⋅ Im'')) γ
+    iPoseProof (own_valid with "HInt") as "%".
+    iMod (own_updateP (flowint_update_P K_multiset I4 (Ip' ⋅ In') (Ip'' ⋅ In'' ⋅ Im'')) γ
                           (● I4 ⋅ ◯ (Ip' ⋅ In')) with "[HInt H']") as (Io'') "H0".
-    { apply (flowint_update I4 (Ip' ⋅ In') (Ip'' ⋅ In'' ⋅ Im'')). done. }
+    {
+      admit.                    (* TODO need to debug *)
+      (* apply (flowint_update K_multiset I4 (Ip' ⋅ In') (Ip'' ⋅ In'' ⋅ Im'')). done. *)
+    }
     { try repeat rewrite own_op; iFrame. rewrite auth_frag_op. rewrite own_op. iFrame.  }
     iPoseProof ((flowint_update_result γ I4 (Ip' ⋅ In') (Ip'' ⋅ In'' ⋅ Im''))
                       with "H0") as (I') "(% & % & HIIpnm)".
     iEval (rewrite own_op) in "HIIpnm". iDestruct "HIIpnm" as "(HI' & HIpnm'')".
     iPoseProof ((own_valid γ (● I')) with "HI'") as "%".
     iPoseProof (own_valid with "HIpnm''") as "%".
-    assert (✓ (Ip'' ⋅ In'' ⋅ Im'')) as HIpnmcheck. 
+    assert (✓ (Ip'' ⋅ In'' ⋅ Im'')) as HIpnmcheck.
     { apply (auth_frag_valid (◯ (Ip'' ⋅ In'' ⋅ Im''))). done. }
     iDestruct "HIpnm''" as "(HIpn'' & HIm'')".
     iPoseProof (own_valid with "HIpn''") as "%".
-    assert (✓ (Ip'' ⋅ In'')) as HIpncheck. 
+    assert (✓ (Ip'' ⋅ In'')) as HIpncheck.
     { apply (auth_frag_valid (◯ (Ip'' ⋅ In''))). done. }
     iDestruct "HIpn''" as "(HIp'' & HIn'')".
     destruct (decide (m ∈ domm I4)). { rewrite (big_sepS_elem_of_acc _ (domm I4) m); last by eauto.
@@ -688,21 +717,31 @@ Section Coupling_Template.
     exfalso. done. }
     iMod (own_update γ_fp (● domm I4) (● (domm I4 ∪ {[m]}) ⋅ ◯ (domm I4 ∪ {[m]})) with "[HFP]") as "H".
     { apply (auth_update_alloc (domm I4) (domm I4 ∪ {[m]}) (domm I4 ∪ {[m]})).
-      apply gset_local_update. set_solver. } done. iDestruct "H" as "(HFP & #Hfp4)".
-      assert (domm I' = domm I4 ∪ {[m]}). { destruct H61 as [I_o H61]. destruct H61.
-      apply flowint_comp_fp in H61. apply flowint_comp_fp in H65.
-      assert (domm (Ip' ⋅ In') = domm Ip' ∪ domm In'). apply flowint_comp_fp. done. done. rewrite H66 in H61.
-      assert (domm (Ip'' ⋅ In'' ⋅ Im'') = domm (Ip'' ⋅ In'') ∪ domm Im''). apply flowint_comp_fp. done. done.
-      rewrite H67 in H65. assert (domm (Ip'' ⋅ In'') = domm Ip'' ∪ domm In''). apply flowint_comp_fp. done. done.
-      rewrite H68 in H65. replace (domm I4). 
-      assert (domm I_o ∪ domm Im'' = domm Im'' ∪ domm I_o). set_solver. replace (domm I').
-      replace (domm In''). replace (domm Ip'). replace (domm In'). replace (domm Ip'').
-      replace (domm Im''). clear. set_solver. apply (auth_auth_valid (I')). done.
-      apply (auth_auth_valid (I4)). done. }
-    assert (globalinv first I'). { by apply (contextualLeq_impl_globalinv I4 I'). }
+      apply gset_local_update. set_solver. }
+    done. iDestruct "H" as "(HFP & #Hfp4)".
+    assert (domm I' = domm I4 ∪ {[m]}).
+    {
+      destruct H61 as [I_o H61]. destruct H61.
+      assert (domm I' = {[p']} ∪ {[n']} ∪ {[m]} ∪ domm I_o).
+      {
+        subst I'. repeat rewrite flowint_comp_fp; try congruence; try done.
+        by apply (auth_auth_valid).
+      }
+      rewrite H66.
+      assert (domm I4 = {[p']} ∪ {[n']} ∪ domm I_o).
+      {
+        subst I4. repeat rewrite flowint_comp_fp; try congruence; try done.
+        by apply (auth_auth_valid).
+      }
+      rewrite H67.
+      (* TODO HELP: how do I ask Coq to use Commutativity? rewrite union_comm. doesn't seem to work. *)
+      admit.
+    }
+    
+    assert (globalinv K first I'). { by apply (contextualLeq_impl_globalinv I4 I'). }
     iEval (rewrite <-H65) in "HFP". assert (domm I'∖ {[m]} = domm I4). { set_solver. }
 
-    (* ------ updates over -------*)  
+    (* ------ updates over -------*)
 
     iMod ("Hclose" with "[Hc]") as "HΦ". iFrame "∗ % #".
     iModIntro. iSplitL "Hstar Hlm Hnodem' HKS Hcont HI' HIm'' HFP Hksm'". iNext. iExists I', C4'.
@@ -710,9 +749,9 @@ Section Coupling_Template.
     iFrame. iExists false. iEval (rewrite H24). iFrame. iExists Im'', Cm''. eauto with iFrame.
     iModIntro. wp_pures. wp_bind (unlockNode _)%E.
 
-    (* ------ linearization over -------*)  
+    (* ------ linearization over -------*)
 
-    awp_apply (unlockNode_spec n') without "HΦ".
+    awp_apply (unlockNode_spec p') without "HΦ".
     iInv "HInv" as ">H". iDestruct "H" as (I5 C5) "(HKS & HInt & % & HFP & Hcont & Hstar)".
     iAssert (⌜n' ∈ domm I5⌝)%I with "[HFP]" as "%".
     { iPoseProof ((auth_set_incl γ_fp Ns (domm I5)) with "[$]") as "%".
@@ -720,11 +759,11 @@ Section Coupling_Template.
     rewrite (big_sepS_elem_of_acc _ (domm I5) n'); last by eauto.
     iDestruct "Hstar" as "[Hb Hstar]". iDestruct "Hb" as (b) "[Hlock Hb]".
     destruct b; last first. { iDestruct "Hb" as (In0 Cn0) "(_ & _ & Hrep' & _)".
-    iAssert (⌜False⌝)%I with "[Hnoden' Hrep']" as %Hf. { iApply (node_sep_star n' In'' In0 _ _ _). 
+    iAssert (⌜False⌝)%I with "[Hnoden' Hrep']" as %Hf. { iApply (node_sep_star n' In'' In0 _ _ _).
     iFrame. } exfalso. done. }
-    iAaccIntro with "Hlock". { iIntros. iModIntro. iFrame "∗ # %". iNext. iExists I5, C5.  
+    iAaccIntro with "Hlock". { iIntros. iModIntro. iFrame "∗ # %". iNext. iExists I5, C5.
     iFrame "∗ # %". iApply "Hstar". iExists true. iFrame. }
-    iIntros. iModIntro. iSplitR "Hnodep' Hksp' HIp''". iNext. iExists I5, C5. 
+    iIntros. iModIntro. iSplitR "Hnodep' Hksp' HIp''". iNext. iExists I5, C5.
     iFrame "∗ # %". iApply "Hstar". iExists false. iFrame. iExists In'', Cn''. iFrame "∗ %".
     iIntros "HΦ". wp_pures. wp_bind (unlockNode _)%E.
     awp_apply (unlockNode_spec p') without "HΦ". iInv "HInv" as ">H".
@@ -735,11 +774,11 @@ Section Coupling_Template.
     rewrite (big_sepS_elem_of_acc _ (domm I6) p'); last by eauto.
     iDestruct "Hstar" as "[Hb Hstar]". iDestruct "Hb" as (b) "[Hlock Hb]".
     destruct b; last first. { iDestruct "Hb" as (In0 Cn0) "(_ & _ & Hrep' & _)".
-    iAssert (⌜False⌝)%I with "[Hnodep' Hrep']" as %Hf. { iApply (node_sep_star p' Ip'' In0 _ _ _). 
+    iAssert (⌜False⌝)%I with "[Hnodep' Hrep']" as %Hf. { iApply (node_sep_star p' Ip'' In0 _ _ _).
     iFrame. } exfalso. done. }
-    iAaccIntro with "Hlock". { iIntros. iModIntro. iFrame "∗". iNext. iExists I6, C6.  
+    iAaccIntro with "Hlock". { iIntros. iModIntro. iFrame "∗". iNext. iExists I6, C6.
     iFrame "∗ # %". iApply "Hstar". iExists true. iFrame. }
-    iIntros. iModIntro. iSplitL. iNext. iExists I6, C6. 
+    iIntros. iModIntro. iSplitL. iNext. iExists I6, C6.
     iFrame "∗ # %". iApply "Hstar". iExists false. iFrame. iExists Ip'', Cp''. iFrame "∗ %".
     iIntros "HΦ". wp_pures. done.
   Qed.
